src/HOL/Auth/Kerberos_BAN.thy
@@ -3,22 +3,23 @@
     Author:     Giampaolo Bella, Cambridge University Computer Laboratory
     Copyright   1998  University of Cambridge
 
-The Kerberos protocol, BAN version.
-
-From page 251 of
-  Burrows, Abadi and Needham.  A Logic of Authentication.
-  Proc. Royal Soc. 426 (1989)
-
-  Confidentiality (secrecy) and authentication properties rely on 
-  temporal checks: strong guarantees in a little abstracted - but
-  very realistic - model (see .thy).
-
 Tidied and converted to Isar by lcp.
 *)
 
-theory Kerberos_BAN = Shared:
+header{*The Kerberos Protocol, BAN Version*}
 
-(* Temporal modelization: session keys can be leaked 
+theory Kerberos_BAN = Public:
+
+text{*From page 251 of
+  Burrows, Abadi and Needham (1989).  A Logic of Authentication.
+  Proc. Royal Soc. 426
+
+  Confidentiality (secrecy) and authentication properties rely on
+  temporal checks: strong guarantees in a little abstracted - but
+  very realistic - model.
+*}
+
+(* Temporal modelization: session keys can be leaked
                           ONLY when they have expired *)
 
 syntax
@@ -46,15 +47,15 @@ specification (AutLife)
 
 
 translations
-   "CT" == "length"
-  
+   "CT" == "length "
+
    "Expired T evs" == "SesKeyLife + T < CT evs"
 
    "RecentAuth T evs" == "CT evs \<le> AutLife + T"
 
 consts  kerberos_ban   :: "event list set"
 inductive "kerberos_ban"
- intros 
+ intros
 
    Nil:  "[] \<in> kerberos_ban"
 
@@ -67,53 +68,53 @@ inductive "kerberos_ban"
 		\<in>  kerberos_ban"
 
 
-   Kb2:  "[| evs2 \<in> kerberos_ban;  Key KAB \<notin> used evs2;
+   Kb2:  "[| evs2 \<in> kerberos_ban;  Key KAB \<notin> used evs2;  KAB \<in> symKeys;
 	     Says A' Server {|Agent A, Agent B|} \<in> set evs2 |]
-	  ==> Says Server A 
+	  ==> Says Server A
 		(Crypt (shrK A)
-		   {|Number (CT evs2), Agent B, Key KAB,  
-		    (Crypt (shrK B) {|Number (CT evs2), Agent A, Key KAB|})|}) 
+		   {|Number (CT evs2), Agent B, Key KAB,
+		    (Crypt (shrK B) {|Number (CT evs2), Agent A, Key KAB|})|})
 		# evs2 \<in> kerberos_ban"
 
 
-   Kb3:  "[| evs3 \<in> kerberos_ban;  
-	     Says S A (Crypt (shrK A) {|Number Ts, Agent B, Key K, X|}) 
+   Kb3:  "[| evs3 \<in> kerberos_ban;
+	     Says S A (Crypt (shrK A) {|Number Ts, Agent B, Key K, X|})
 	       \<in> set evs3;
 	     Says A Server {|Agent A, Agent B|} \<in> set evs3;
 	     ~ Expired Ts evs3 |]
-	  ==> Says A B {|X, Crypt K {|Agent A, Number (CT evs3)|} |} 
+	  ==> Says A B {|X, Crypt K {|Agent A, Number (CT evs3)|} |}
 	       # evs3 \<in> kerberos_ban"
 
 
-   Kb4:  "[| evs4 \<in> kerberos_ban;  
-	     Says A' B {|(Crypt (shrK B) {|Number Ts, Agent A, Key K|}), 
+   Kb4:  "[| evs4 \<in> kerberos_ban;
+	     Says A' B {|(Crypt (shrK B) {|Number Ts, Agent A, Key K|}),
 			 (Crypt K {|Agent A, Number Ta|}) |}: set evs4;
 	     ~ Expired Ts evs4;  RecentAuth Ta evs4 |]
 	  ==> Says B A (Crypt K (Number Ta)) # evs4
 		\<in> kerberos_ban"
 
 	(*Old session keys may become compromised*)
-   Oops: "[| evso \<in> kerberos_ban;  
+   Oops: "[| evso \<in> kerberos_ban;
 	     Says Server A (Crypt (shrK A) {|Number Ts, Agent B, Key K, X|})
 	       \<in> set evso;
 	     Expired Ts evso |]
 	  ==> Notes Spy {|Number Ts, Key K|} # evso \<in> kerberos_ban"
 
 
-declare Says_imp_knows_Spy [THEN parts.Inj, dest] 
+declare Says_imp_knows_Spy [THEN parts.Inj, dest]
 declare parts.Body [dest]
 declare analz_into_parts [dest]
 declare Fake_parts_insert_in_Un [dest]
 
-(*A "possibility property": there are traces that reach the end.*)
-lemma "Key K \<notin> used []
-       ==> \<exists>Timestamp. \<exists>evs \<in> kerberos_ban.     
-             Says B A (Crypt K (Number Timestamp))  
+text{*A "possibility property": there are traces that reach the end.*}
+lemma "[|Key K \<notin> used []; K \<in> symKeys|]
+       ==> \<exists>Timestamp. \<exists>evs \<in> kerberos_ban.
+             Says B A (Crypt K (Number Timestamp))
                   \<in> set evs"
 apply (cut_tac SesKeyLife_LB)
 apply (intro exI bexI)
-apply (rule_tac [2] 
-           kerberos_ban.Nil [THEN kerberos_ban.Kb1, THEN kerberos_ban.Kb2, 
+apply (rule_tac [2]
+           kerberos_ban.Nil [THEN kerberos_ban.Kb1, THEN kerberos_ban.Kb2,
                              THEN kerberos_ban.Kb3, THEN kerberos_ban.Kb4])
 apply (possibility, simp_all (no_asm_simp) add: used_Cons)
 done
@@ -121,114 +122,109 @@ done
 
 (**** Inductive proofs about kerberos_ban ****)
 
-(*Forwarding Lemma for reasoning about the encrypted portion of message Kb3*)
+text{*Forwarding Lemma for reasoning about the encrypted portion of message Kb3*}
 lemma Kb3_msg_in_parts_spies:
-     "Says S A (Crypt KA {|Timestamp, B, K, X|}) \<in> set evs  
+     "Says S A (Crypt KA {|Timestamp, B, K, X|}) \<in> set evs
       ==> X \<in> parts (spies evs)"
 by blast
-                              
+
 lemma Oops_parts_spies:
-     "Says Server A (Crypt (shrK A) {|Timestamp, B, K, X|}) \<in> set evs  
+     "Says Server A (Crypt (shrK A) {|Timestamp, B, K, X|}) \<in> set evs
       ==> K \<in> parts (spies evs)"
 by blast
 
 
-(*Spy never sees another agent's shared key! (unless it's bad at start)*)
+text{*Spy never sees another agent's shared key! (unless it's bad at start)*}
 lemma Spy_see_shrK [simp]:
      "evs \<in> kerberos_ban ==> (Key (shrK A) \<in> parts (spies evs)) = (A \<in> bad)"
-apply (erule kerberos_ban.induct) 
-apply (frule_tac [7] Oops_parts_spies) 
-apply (frule_tac [5] Kb3_msg_in_parts_spies, simp_all)  
-apply blast+
+apply (erule kerberos_ban.induct)
+apply (frule_tac [7] Oops_parts_spies)
+apply (frule_tac [5] Kb3_msg_in_parts_spies, simp_all, blast+)
 done
 
 
 lemma Spy_analz_shrK [simp]:
      "evs \<in> kerberos_ban ==> (Key (shrK A) \<in> analz (spies evs)) = (A \<in> bad)"
-apply auto
-done
-
+by auto
 
 lemma Spy_see_shrK_D [dest!]:
-     "[| Key (shrK A) \<in> parts (spies evs);        
+     "[| Key (shrK A) \<in> parts (spies evs);
                 evs \<in> kerberos_ban |] ==> A:bad"
-apply (blast dest: Spy_see_shrK)
-done
+by (blast dest: Spy_see_shrK)
 
 lemmas Spy_analz_shrK_D = analz_subset_parts [THEN subsetD, THEN Spy_see_shrK_D,  dest!]
 
 
-(*Nobody can have used non-existent keys!*)
-lemma new_keys_not_used [rule_format, simp]:
-     "evs \<in> kerberos_ban ==>       
-       Key K \<notin> used evs --> K \<notin> keysFor (parts (spies evs))"
-apply (erule kerberos_ban.induct) 
-apply (frule_tac [7] Oops_parts_spies) 
-apply (frule_tac [5] Kb3_msg_in_parts_spies, simp_all)  
-(*Fake*)
+text{*Nobody can have used non-existent keys!*}
+lemma new_keys_not_used [simp]:
+    "[|Key K \<notin> used evs; K \<in> symKeys; evs \<in> kerberos_ban|]
+     ==> K \<notin> keysFor (parts (spies evs))"
+apply (erule rev_mp)
+apply (erule kerberos_ban.induct)
+apply (frule_tac [7] Oops_parts_spies)
+apply (frule_tac [5] Kb3_msg_in_parts_spies, simp_all)
+txt{*Fake*}
 apply (force dest!: keysFor_parts_insert)
-(*Kb2, Kb3, Kb4*)
-apply blast+
+txt{*Kb2, Kb3, Kb4*}
+apply (force dest!: analz_shrK_Decrypt)+
 done
 
-(** Lemmas concerning the form of items passed in messages **)
+subsection{* Lemmas concerning the form of items passed in messages *}
 
-(*Describes the form of K, X and K' when the Server sends this message.*)
+text{*Describes the form of K, X and K' when the Server sends this message.*}
 lemma Says_Server_message_form:
-     "[| Says Server A (Crypt K' {|Number Ts, Agent B, Key K, X|})   
-         \<in> set evs; evs \<in> kerberos_ban |]                            
-      ==> K \<notin> range shrK &                                          
-          X = (Crypt (shrK B) {|Number Ts, Agent A, Key K|}) &       
+     "[| Says Server A (Crypt K' {|Number Ts, Agent B, Key K, X|})
+         \<in> set evs; evs \<in> kerberos_ban |]
+      ==> K \<notin> range shrK &
+          X = (Crypt (shrK B) {|Number Ts, Agent A, Key K|}) &
           K' = shrK A"
 apply (erule rev_mp)
 apply (erule kerberos_ban.induct, auto)
 done
 
 
-(*If the encrypted message appears then it originated with the Server
+text{*If the encrypted message appears then it originated with the Server
   PROVIDED that A is NOT compromised!
 
   This shows implicitly the FRESHNESS OF THE SESSION KEY to A
-*)
+*}
 lemma A_trusts_K_by_Kb2:
-     "[| Crypt (shrK A) {|Number Ts, Agent B, Key K, X|}  
-           \<in> parts (spies evs);                           
-         A \<notin> bad;  evs \<in> kerberos_ban |]                 
-       ==> Says Server A (Crypt (shrK A) {|Number Ts, Agent B, Key K, X|})  
+     "[| Crypt (shrK A) {|Number Ts, Agent B, Key K, X|}
+           \<in> parts (spies evs);
+         A \<notin> bad;  evs \<in> kerberos_ban |]
+       ==> Says Server A (Crypt (shrK A) {|Number Ts, Agent B, Key K, X|})
              \<in> set evs"
 apply (erule rev_mp)
-apply (erule kerberos_ban.induct) 
-apply (frule_tac [7] Oops_parts_spies) 
-apply (frule_tac [5] Kb3_msg_in_parts_spies, simp_all)  
-apply blast
+apply (erule kerberos_ban.induct)
+apply (frule_tac [7] Oops_parts_spies)
+apply (frule_tac [5] Kb3_msg_in_parts_spies, simp_all, blast)
 done
 
 
-(*If the TICKET appears then it originated with the Server*)
-(*FRESHNESS OF THE SESSION KEY to B*)
+text{*If the TICKET appears then it originated with the Server*}
+text{*FRESHNESS OF THE SESSION KEY to B*}
 lemma B_trusts_K_by_Kb3:
-     "[| Crypt (shrK B) {|Number Ts, Agent A, Key K|} \<in> parts (spies evs);  
-         B \<notin> bad;  evs \<in> kerberos_ban |]                         
-       ==> Says Server A                                          
-            (Crypt (shrK A) {|Number Ts, Agent B, Key K,                    
-                          Crypt (shrK B) {|Number Ts, Agent A, Key K|}|})   
+     "[| Crypt (shrK B) {|Number Ts, Agent A, Key K|} \<in> parts (spies evs);
+         B \<notin> bad;  evs \<in> kerberos_ban |]
+       ==> Says Server A
+            (Crypt (shrK A) {|Number Ts, Agent B, Key K,
+                          Crypt (shrK B) {|Number Ts, Agent A, Key K|}|})
            \<in> set evs"
 apply (erule rev_mp)
-apply (erule kerberos_ban.induct) 
-apply (frule_tac [7] Oops_parts_spies) 
-apply (frule_tac [5] Kb3_msg_in_parts_spies, simp_all)  
-apply blast
+apply (erule kerberos_ban.induct)
+apply (frule_tac [7] Oops_parts_spies)
+apply (frule_tac [5] Kb3_msg_in_parts_spies, simp_all, blast)
 done
 
 
-(*EITHER describes the form of X when the following message is sent, 
+text{*EITHER describes the form of X when the following message is sent,
   OR     reduces it to the Fake case.
-  Use Says_Server_message_form if applicable.*)
+  Use @{text Says_Server_message_form} if applicable.*}
 lemma Says_S_message_form:
-     "[| Says S A (Crypt (shrK A) {|Number Ts, Agent B, Key K, X|})      
-            \<in> set evs;                                                   
-         evs \<in> kerberos_ban |]                                           
- ==> (K \<notin> range shrK & X = (Crypt (shrK B) {|Number Ts, Agent A, Key K|})) 
+     "[| Says S A (Crypt (shrK A) {|Number Ts, Agent B, Key K, X|})
+            \<in> set evs;
+         evs \<in> kerberos_ban |]
+ ==> (K \<notin> range shrK & X = (Crypt (shrK B) {|Number Ts, Agent A, Key K|}))
           | X \<in> analz (spies evs)"
 apply (case_tac "A \<in> bad")
 apply (force dest!: Says_imp_spies [THEN analz.Inj])
@@ -248,56 +244,51 @@ done
 
 ****)
 
-
-(** Session keys are not used to encrypt other session keys **)
-
+text{* Session keys are not used to encrypt other session keys *}
 lemma analz_image_freshK [rule_format (no_asm)]:
-     "evs \<in> kerberos_ban ==>                           
-   \<forall>K KK. KK \<subseteq> - (range shrK) -->                  
-          (Key K \<in> analz (Key`KK Un (spies evs))) =   
+     "evs \<in> kerberos_ban ==>
+   \<forall>K KK. KK \<subseteq> - (range shrK) -->
+          (Key K \<in> analz (Key`KK Un (spies evs))) =
           (K \<in> KK | Key K \<in> analz (spies evs))"
 apply (erule kerberos_ban.induct)
 apply (drule_tac [7] Says_Server_message_form)
-apply (erule_tac [5] Says_S_message_form [THEN disjE], analz_freshK, spy_analz)
+apply (erule_tac [5] Says_S_message_form [THEN disjE], analz_freshK, spy_analz, auto) 
 done
 
 
-
 lemma analz_insert_freshK:
-     "[| evs \<in> kerberos_ban;  KAB \<notin> range shrK |] ==>      
-      (Key K \<in> analz (insert (Key KAB) (spies evs))) =        
+     "[| evs \<in> kerberos_ban;  KAB \<notin> range shrK |] ==>
+      (Key K \<in> analz (insert (Key KAB) (spies evs))) =
       (K = KAB | Key K \<in> analz (spies evs))"
 by (simp only: analz_image_freshK analz_image_freshK_simps)
 
 
-(** The session key K uniquely identifies the message **)
-
+text{* The session key K uniquely identifies the message *}
 lemma unique_session_keys:
-     "[| Says Server A                                     
-           (Crypt (shrK A) {|Number Ts, Agent B, Key K, X|}) \<in> set evs;   
-         Says Server A'                                    
-          (Crypt (shrK A') {|Number Ts', Agent B', Key K, X'|}) \<in> set evs; 
+     "[| Says Server A
+           (Crypt (shrK A) {|Number Ts, Agent B, Key K, X|}) \<in> set evs;
+         Says Server A'
+          (Crypt (shrK A') {|Number Ts', Agent B', Key K, X'|}) \<in> set evs;
          evs \<in> kerberos_ban |] ==> A=A' & Ts=Ts' & B=B' & X = X'"
 apply (erule rev_mp)
 apply (erule rev_mp)
-apply (erule kerberos_ban.induct) 
-apply (frule_tac [7] Oops_parts_spies) 
-apply (frule_tac [5] Kb3_msg_in_parts_spies, simp_all)  
-(*Kb2: it can't be a new key*)
+apply (erule kerberos_ban.induct)
+apply (frule_tac [7] Oops_parts_spies)
+apply (frule_tac [5] Kb3_msg_in_parts_spies, simp_all)
+txt{*Kb2: it can't be a new key*}
 apply blast
 done
 
 
-(** Lemma: the session key sent in msg Kb2 would be EXPIRED
-    if the spy could see it!
-**)
+text{* Lemma: the session key sent in msg Kb2 would be EXPIRED
+    if the spy could see it! *}
 
 lemma lemma2 [rule_format (no_asm)]:
-     "[| A \<notin> bad;  B \<notin> bad;  evs \<in> kerberos_ban |]            
-  ==> Says Server A                                             
-          (Crypt (shrK A) {|Number Ts, Agent B, Key K,          
-                            Crypt (shrK B) {|Number Ts, Agent A, Key K|}|}) 
-         \<in> set evs -->                                          
+     "[| A \<notin> bad;  B \<notin> bad;  evs \<in> kerberos_ban |]
+  ==> Says Server A
+          (Crypt (shrK A) {|Number Ts, Agent B, Key K,
+                            Crypt (shrK B) {|Number Ts, Agent A, Key K|}|})
+         \<in> set evs -->
       Key K \<in> analz (spies evs) --> Expired Ts evs"
 apply (erule kerberos_ban.induct)
 apply (frule_tac [7] Says_Server_message_form)
@@ -316,54 +307,48 @@ apply (blast dest: unique_session_keys intro!: less_SucI)
 done
 
 
-(** CONFIDENTIALITY for the SERVER:
-                     Spy does not see the keys sent in msg Kb2 
-                     as long as they have NOT EXPIRED
-**)
+text{*Confidentiality for the Server: Spy does not see the keys sent in msg Kb2
+as long as they have not expired.*}
 lemma Confidentiality_S:
-     "[| Says Server A                                            
-          (Crypt K' {|Number T, Agent B, Key K, X|}) \<in> set evs;   
-         ~ Expired T evs;                                         
-         A \<notin> bad;  B \<notin> bad;  evs \<in> kerberos_ban                 
+     "[| Says Server A
+          (Crypt K' {|Number T, Agent B, Key K, X|}) \<in> set evs;
+         ~ Expired T evs;
+         A \<notin> bad;  B \<notin> bad;  evs \<in> kerberos_ban
       |] ==> Key K \<notin> analz (spies evs)"
 apply (frule Says_Server_message_form, assumption)
 apply (blast intro: lemma2)
 done
 
-(**** THE COUNTERPART OF CONFIDENTIALITY 
+(**** THE COUNTERPART OF CONFIDENTIALITY
       [|...; Expired Ts evs; ...|] ==> Key K \<in> analz (spies evs)
       WOULD HOLD ONLY IF AN OOPS OCCURRED! ---> Nothing to prove!   ****)
 
 
-(** CONFIDENTIALITY for ALICE: **)
-(** Also A_trusts_K_by_Kb2 RS Confidentiality_S **)
+text{*Confidentiality for Alice*}
 lemma Confidentiality_A:
-     "[| Crypt (shrK A) {|Number T, Agent B, Key K, X|} \<in> parts (spies evs); 
-         ~ Expired T evs;           
-         A \<notin> bad;  B \<notin> bad;  evs \<in> kerberos_ban                 
+     "[| Crypt (shrK A) {|Number T, Agent B, Key K, X|} \<in> parts (spies evs);
+         ~ Expired T evs;
+         A \<notin> bad;  B \<notin> bad;  evs \<in> kerberos_ban
       |] ==> Key K \<notin> analz (spies evs)"
-apply (blast dest!: A_trusts_K_by_Kb2 Confidentiality_S)
-done
+by (blast dest!: A_trusts_K_by_Kb2 Confidentiality_S)
 
 
-(** CONFIDENTIALITY for BOB: **)
-(** Also B_trusts_K_by_Kb3 RS Confidentiality_S **)
+text{*Confidentiality for Bob*}
 lemma Confidentiality_B:
-     "[| Crypt (shrK B) {|Number Tk, Agent A, Key K|}  
-          \<in> parts (spies evs);               
-        ~ Expired Tk evs;           
-        A \<notin> bad;  B \<notin> bad;  evs \<in> kerberos_ban                 
+     "[| Crypt (shrK B) {|Number Tk, Agent A, Key K|}
+          \<in> parts (spies evs);
+        ~ Expired Tk evs;
+        A \<notin> bad;  B \<notin> bad;  evs \<in> kerberos_ban
       |] ==> Key K \<notin> analz (spies evs)"
-apply (blast dest!: B_trusts_K_by_Kb3 Confidentiality_S)
-done
+by (blast dest!: B_trusts_K_by_Kb3 Confidentiality_S)
 
 
 lemma lemma_B [rule_format]:
-     "[| B \<notin> bad;  evs \<in> kerberos_ban |]                         
-      ==> Key K \<notin> analz (spies evs) -->                     
-          Says Server A (Crypt (shrK A) {|Number Ts, Agent B, Key K, X|})  
-          \<in> set evs -->                                              
-          Crypt K (Number Ta) \<in> parts (spies evs) -->         
+     "[| B \<notin> bad;  evs \<in> kerberos_ban |]
+      ==> Key K \<notin> analz (spies evs) -->
+          Says Server A (Crypt (shrK A) {|Number Ts, Agent B, Key K, X|})
+          \<in> set evs -->
+          Crypt K (Number Ta) \<in> parts (spies evs) -->
           Says B A (Crypt K (Number Ta)) \<in> set evs"
 apply (erule kerberos_ban.induct)
 apply (frule_tac [7] Oops_parts_spies)
@@ -372,35 +357,33 @@ apply (drule_tac [6] Kb3_msg_in_parts_spies, analz_mono_contra)
 apply (simp_all (no_asm_simp) add: all_conj_distrib)
 txt{*Fake*}
 apply blast
-txt{*Kb2*}
-apply (force dest: Crypt_imp_invKey_keysFor) 
+txt{*Kb2*} 
+apply (force dest: Crypt_imp_invKey_keysFor)
 txt{*Kb4*}
-apply (blast dest: B_trusts_K_by_Kb3 unique_session_keys 
+apply (blast dest: B_trusts_K_by_Kb3 unique_session_keys
                    Says_imp_spies [THEN analz.Inj] Crypt_Spy_analz_bad)
 done
 
 
-(*AUTHENTICATION OF B TO A*)
+text{*Authentication of B to A*}
 lemma Authentication_B:
-     "[| Crypt K (Number Ta) \<in> parts (spies evs);            
-         Crypt (shrK A) {|Number Ts, Agent B, Key K, X|}     
-         \<in> parts (spies evs);                                
-         ~ Expired Ts evs;                                   
-         A \<notin> bad;  B \<notin> bad;  evs \<in> kerberos_ban |]         
+     "[| Crypt K (Number Ta) \<in> parts (spies evs);
+         Crypt (shrK A) {|Number Ts, Agent B, Key K, X|}
+         \<in> parts (spies evs);
+         ~ Expired Ts evs;
+         A \<notin> bad;  B \<notin> bad;  evs \<in> kerberos_ban |]
       ==> Says B A (Crypt K (Number Ta)) \<in> set evs"
 by (blast dest!: A_trusts_K_by_Kb2
           intro!: lemma_B elim!: Confidentiality_S [THEN [2] rev_notE])
 
-
-
 lemma lemma_A [rule_format]:
-     "[| A \<notin> bad; B \<notin> bad; evs \<in> kerberos_ban |] 
-      ==>           
-         Key K \<notin> analz (spies evs) -->          
-         Says Server A (Crypt (shrK A) {|Number Ts, Agent B, Key K, X|})   
-         \<in> set evs -->   
-          Crypt K {|Agent A, Number Ta|} \<in> parts (spies evs) --> 
-         Says A B {|X, Crypt K {|Agent A, Number Ta|}|}   
+     "[| A \<notin> bad; B \<notin> bad; evs \<in> kerberos_ban |]
+      ==>
+         Key K \<notin> analz (spies evs) -->
+         Says Server A (Crypt (shrK A) {|Number Ts, Agent B, Key K, X|})
+         \<in> set evs -->
+          Crypt K {|Agent A, Number Ta|} \<in> parts (spies evs) -->
+         Says A B {|X, Crypt K {|Agent A, Number Ta|}|}
              \<in> set evs"
 apply (erule kerberos_ban.induct)
 apply (frule_tac [7] Oops_parts_spies)
@@ -410,23 +393,22 @@ apply (simp_all (no_asm_simp) add: all_conj_distrib)
 txt{*Fake*}
 apply blast
 txt{*Kb2*}
-apply (force dest: Crypt_imp_invKey_keysFor) 
+apply (force dest: Crypt_imp_invKey_keysFor)
 txt{*Kb3*}
 apply (blast dest: A_trusts_K_by_Kb2 unique_session_keys)
 done
 
-
-(*AUTHENTICATION OF A TO B*)
+text{*Authentication of A to B*}
 lemma Authentication_A:
-     "[| Crypt K {|Agent A, Number Ta|} \<in> parts (spies evs);   
-         Crypt (shrK B) {|Number Ts, Agent A, Key K|}          
-         \<in> parts (spies evs);                                  
-         ~ Expired Ts evs;                                     
-         A \<notin> bad;  B \<notin> bad;  evs \<in> kerberos_ban |]           
-      ==> Says A B {|Crypt (shrK B) {|Number Ts, Agent A, Key K|},      
+     "[| Crypt K {|Agent A, Number Ta|} \<in> parts (spies evs);
+         Crypt (shrK B) {|Number Ts, Agent A, Key K|}
+         \<in> parts (spies evs);
+         ~ Expired Ts evs;
+         A \<notin> bad;  B \<notin> bad;  evs \<in> kerberos_ban |]
+      ==> Says A B {|Crypt (shrK B) {|Number Ts, Agent A, Key K|},
                      Crypt K {|Agent A, Number Ta|}|} \<in> set evs"
 by (blast dest!: B_trusts_K_by_Kb3
-          intro!: lemma_A 
+          intro!: lemma_A
           elim!: Confidentiality_S [THEN [2] rev_notE])
 
 end
