src/HOL/Auth/OtwayRees_Bad.thy
@@ -2,20 +2,22 @@
     ID:         $Id$
     Author:     Lawrence C Paulson, Cambridge University Computer Laboratory
     Copyright   1996  University of Cambridge
-
-Inductive relation "otway" for the Otway-Rees protocol.
-
-The FAULTY version omitting encryption of Nonce NB, as suggested on page 247 of
-  Burrows, Abadi and Needham.  A Logic of Authentication.
-  Proc. Royal Soc. 426 (1989)
-
-This file illustrates the consequences of such errors.  We can still prove
-impressive-looking properties such as Spy_not_see_encrypted_key, yet the
-protocol is open to a middleperson attack.  Attempting to prove some key lemmas
-indicates the possibility of this attack.
 *)
 
-theory OtwayRees_Bad = Shared:
+
+header{*The Otway-Rees Protocol: The Faulty BAN Version*}
+
+theory OtwayRees_Bad = Public:
+
+text{*The FAULTY version omitting encryption of Nonce NB, as suggested on 
+page 247 of
+  Burrows, Abadi and Needham (1988).  A Logic of Authentication.
+  Proc. Royal Soc. 426
+
+This file illustrates the consequences of such errors.  We can still prove
+impressive-looking properties such as @{text Spy_not_see_encrypted_key}, yet
+the protocol is open to a middleperson attack.  Attempting to prove some key
+lemmas indicates the possibility of this attack.*}
 
 consts  otway   :: "event list set"
 inductive "otway"
@@ -184,10 +186,10 @@ lemma analz_image_freshK [rule_format]:
    \<forall>K KK. KK <= -(range shrK) -->
           (Key K \<in> analz (Key`KK Un (knows Spy evs))) =
           (K \<in> KK | Key K \<in> analz (knows Spy evs))"
-apply (erule otway.induct, force)
-apply (frule_tac [7] Says_Server_message_form)
-apply (drule_tac [6] OR4_analz_knows_Spy)
-apply (drule_tac [4] OR2_analz_knows_Spy, analz_freshK, spy_analz)
+apply (erule otway.induct)
+apply (frule_tac [8] Says_Server_message_form)
+apply (drule_tac [7] OR4_analz_knows_Spy)
+apply (drule_tac [5] OR2_analz_knows_Spy, analz_freshK, spy_analz, auto) 
 done
 
 lemma analz_insert_freshK:
